isabelle: Remove the no-shadowing rule for Core.

isabelle/core/CoreTyEnv.thy
@@ -29,8 +29,11 @@ record CoreTyEnv =
      Globals are implicitly constant and do not appear in TE_ConstNames. *)
   TE_GlobalVars :: "(string, CoreType) fmap"
 
-  (* Ghost variables - subset of TE_LocalVars and TE_GlobalVars keys *)
-  TE_GhostVars :: "string fset"
+  (* Ghost local variables - subset of TE_LocalVars keys *)
+  TE_GhostLocals :: "string fset"
+
+  (* Ghost global variables - subset of TE_GlobalVars keys *)
+  TE_GhostGlobals :: "string fset"
 
   (* Constant local names - subset of TE_LocalVars keys; these are not assignable.
      Globals are implicitly constant and do not need to appear here. *)
@@ -68,6 +71,15 @@ record CoreTyEnv =
      contains MathInt, MathReal, or another ghost datatype. *)
   TE_GhostDatatypes :: "string fset"
 
+(* Is a variable ghost? For locals, check TE_GhostLocals; for globals, TE_GhostGlobals.
+   Locals shadow globals, so if a name is in both TE_LocalVars and TE_GlobalVars,
+   only the local ghost status matters. *)
+definition tyenv_var_ghost :: "CoreTyEnv \<Rightarrow> string \<Rightarrow> bool" where
+  "tyenv_var_ghost env name =
+    (case fmlookup (TE_LocalVars env) name of
+      Some _ \<Rightarrow> name |\<in>| TE_GhostLocals env
+    | None \<Rightarrow> name |\<in>| TE_GhostGlobals env)"
+
 (* Look up a term variable: locals shadow globals *)
 definition tyenv_lookup_var :: "CoreTyEnv \<Rightarrow> string \<Rightarrow> CoreType option" where
   "tyenv_lookup_var env name =
@@ -81,16 +93,15 @@ definition tyenv_var_writable :: "CoreTyEnv \<Rightarrow> string \<Rightarrow> b
   "tyenv_var_writable env name =
     (fmlookup (TE_LocalVars env) name \<noteq> None \<and> name |\<notin>| TE_ConstNames env)"
 
-(* tyenv_subset env1 env2: env1 is a "sub-environment" of env2.
-   This means env2 has all the same variables (with the same types) plus possibly more.
-   Only locals may grow; globals and "fixed" fields must be identical. *)
-definition tyenv_subset :: "CoreTyEnv \<Rightarrow> CoreTyEnv \<Rightarrow> bool" where
-  "tyenv_subset env1 env2 \<equiv>
-    (\<forall>name ty. fmlookup (TE_LocalVars env1) name = Some ty \<longrightarrow>
-               fmlookup (TE_LocalVars env2) name = Some ty) \<and>
+(* tyenv_fixed_eq env1 env2: the "fixed" fields of env1 and env2 are identical.
+   These are the fields that do not change during statement execution:
+   globals, ghost globals, return type, function ghost-ness, functions, datatypes, etc.
+   This is used in the Return case of sound_statement_result to transfer
+   value_has_type and TE_ReturnType across environments. *)
+definition tyenv_fixed_eq :: "CoreTyEnv \<Rightarrow> CoreTyEnv \<Rightarrow> bool" where
+  "tyenv_fixed_eq env1 env2 \<equiv>
     TE_GlobalVars env1 = TE_GlobalVars env2 \<and>
-    TE_GhostVars env1 |\<subseteq>| TE_GhostVars env2 \<and>
-    TE_ConstNames env1 |\<subseteq>| TE_ConstNames env2 \<and>
+    TE_GhostGlobals env1 = TE_GhostGlobals env2 \<and>
     TE_ReturnType env1 = TE_ReturnType env2 \<and>
     TE_FunctionGhost env1 = TE_FunctionGhost env2 \<and>
     TE_Functions env1 = TE_Functions env2 \<and>
@@ -101,13 +112,18 @@ definition tyenv_subset :: "CoreTyEnv \<Rightarrow> CoreTyEnv \<Rightarrow> bool
     TE_TypeVars env1 = TE_TypeVars env2 \<and>
     TE_RuntimeTypeVars env1 = TE_RuntimeTypeVars env2"
 
-lemma tyenv_subset_refl: "tyenv_subset env env"
-  unfolding tyenv_subset_def by simp
+lemma tyenv_fixed_eq_refl: "tyenv_fixed_eq env env"
+  unfolding tyenv_fixed_eq_def by simp
 
-lemma tyenv_subset_trans:
-  assumes "tyenv_subset env1 env2" and "tyenv_subset env2 env3"
-  shows "tyenv_subset env1 env3"
-  using assms unfolding tyenv_subset_def by (auto dest: fsubset_trans)
+lemma tyenv_fixed_eq_trans:
+  assumes "tyenv_fixed_eq env1 env2" and "tyenv_fixed_eq env2 env3"
+  shows "tyenv_fixed_eq env1 env3"
+  using assms unfolding tyenv_fixed_eq_def by simp
+
+lemma tyenv_fixed_eq_sym:
+  assumes "tyenv_fixed_eq env1 env2"
+  shows "tyenv_fixed_eq env2 env1"
+  using assms unfolding tyenv_fixed_eq_def by simp
 
 lemma tyenv_lookup_var_local [simp]:
   "fmlookup (TE_LocalVars env) name = Some ty \<Longrightarrow> tyenv_lookup_var env name = Some ty"
@@ -122,5 +138,8 @@ lemma tyenv_lookup_var_TE_ConstNames_irrelevant [simp]:
   "tyenv_lookup_var (env \<lparr> TE_ConstNames := c \<rparr>) name = tyenv_lookup_var env name"
   unfolding tyenv_lookup_var_def by (simp split: option.splits)
 
+lemma tyenv_var_ghost_TE_ConstNames_irrelevant [simp]:
+  "tyenv_var_ghost (env \<lparr> TE_ConstNames := c \<rparr>) name = tyenv_var_ghost env name"
+  unfolding tyenv_var_ghost_def by (simp split: option.splits)
 
 end
